frodo/code/Hacl.Impl.Frodo.KEM.Encaps.fst
@@ -429,7 +429,6 @@ let crypto_kem_enc_ coins ct ss pk =
   push_frame();
   let bytes_mu = params_nbar *! params_nbar *! params_extracted_bits /. size 8 in
   let g:lbytes (size 3 *! crypto_bytes) = create (size 3 *! crypto_bytes) (u8 0) in
-
   crypto_kem_enc_0 coins pk g;
   crypto_kem_enc_1 g coins ct ss pk;
   pop_frame()
@@ -441,11 +440,12 @@ val crypto_kem_enc:
   -> pk:lbytes crypto_publickeybytes
   -> Stack uint32
     (requires fun h ->
+      live h state /\ disjoint state ct /\ disjoint state ss /\ disjoint state pk /\
       live h ct /\ live h ss /\ live h pk /\
       disjoint ct ss /\ disjoint ct pk /\ disjoint ss pk)
     (ensures  fun h0 _ h1 ->
-      modifies (loc_union (loc_buffer ct) (loc_buffer ss)) h0 h1 /\
-      (let ct_s, ss_s = S.crypto_kem_enc (as_seq h0 pk) in
+      modifies (loc_union (loc_buffer state) (loc_union (loc_buffer ct) (loc_buffer ss))) h0 h1 /\
+      (let ct_s, ss_s = S.crypto_kem_enc (as_seq h0 state) (as_seq h0 pk) in
       as_seq h1 ct == ct_s /\ as_seq h1 ss == ss_s))
 let crypto_kem_enc ct ss pk =
   push_frame();
