frodo/code/Hacl.Impl.Frodo.KEM.KeyGen.fst
@@ -157,10 +157,12 @@ val crypto_kem_keypair:
     pk:lbytes crypto_publickeybytes
   -> sk:lbytes crypto_secretkeybytes
   -> Stack uint32
-    (requires fun h -> live h pk /\ live h sk /\ disjoint pk sk)
+    (requires fun h ->
+      live h state /\ disjoint state pk /\ disjoint state sk /\
+      live h pk /\ live h sk /\ disjoint pk sk)
     (ensures  fun h0 r h1 ->
-      modifies (loc_union (loc_buffer pk) (loc_buffer sk)) h0 h1 /\
-      (let pk_s, sk_s = S.crypto_kem_keypair () in
+      modifies (loc_union (loc_buffer state) (loc_union (loc_buffer pk) (loc_buffer sk))) h0 h1 /\
+      (let pk_s, sk_s = S.crypto_kem_keypair (as_seq h0 state) in
       as_seq h1 pk == pk_s /\ as_seq h1 sk == sk_s))
 let crypto_kem_keypair pk sk =
   push_frame();
